Sitpn/SitpnCorrect.v
@@ -1,0 +1,49 @@
+(* Import Sitpn material. *)
+
+Require Import Hilecop.Sitpn.Sitpn.
+Require Import Hilecop.Sitpn.SitpnTokenPlayer.
+Require Import Hilecop.Sitpn.SitpnSemantics.
+
+(* Import falling edge correctness lemmas. *)
+
+Require Import Hilecop.Sitpn.SitpnFallingEdgeCorrect.
+Require Import Hilecop.Sitpn.SitpnFallingEdgeWellDef.
+
+(* Import rising edge correctness lemmas. *)
+
+Require Import Hilecop.Sitpn.SitpnRisingEdgeCorrect.
+
+(** * Correctness theorem for SITPN token player program. *)
+
+Theorem sitpn_cycle_correct :
+  forall (sitpn : Sitpn)
+         (s s' s'' : SitpnState)
+         (time_value : nat)
+         (env : Condition -> nat -> bool),
+    IsWellDefinedSitpn sitpn ->
+    IsWellDefinedSitpnState sitpn s ->
+    sitpn_cycle sitpn s time_value env = Some (s', s'') ->
+    SitpnSemantics sitpn s s' time_value env falling_edge /\
+    SitpnSemantics sitpn s' s'' time_value env rising_edge.
+Proof.
+  intros sitpn s s' s'' time_value env Hwell_def_sitpn Hwell_def_s Hfun.
+  functional induction (sitpn_cycle sitpn s time_value env) using sitpn_cycle_ind.
+  (* GENERAL CASE, all went well. *)
+  - injection Hfun as Heq_s' Heq_s''.
+    split.
+    (* CASE falling edge correct. *)
+    + rewrite <- Heq_s'.
+      apply (sitpn_falling_edge_correct sitpn s s'0 time_value env
+                                        Hwell_def_sitpn Hwell_def_s e).
+    (* CASE rising edge correct. *)
+    + specialize (sitpn_falling_edge_well_def_state
+                    sitpn s s'0 time_value env Hwell_def_sitpn Hwell_def_s e)
+        as Hwell_def_s'.
+      rewrite <- Heq_s', <- Heq_s''.
+      apply (sitpn_rising_edge_correct
+               sitpn s'0 s''0 time_value env Hwell_def_sitpn Hwell_def_s' e0). 
+  (* Error case. *)
+  - inversion Hfun.
+  (* Error case. *)
+  - inversion Hfun.
+Qed.
