Sitpn/SitpnFallingEdgeCorrect.v
@@ -1,0 +1,73 @@
+(* Import Sitpn material. *)
+
+Require Import Hilecop.Sitpn.Sitpn.
+Require Import Hilecop.Sitpn.SitpnTokenPlayer.
+Require Import Hilecop.Sitpn.SitpnSemantics.
+
+(* Import sitpn falling edge well-defined state. *)
+
+Require Import Hilecop.Sitpn.SitpnFallingEdgeWellDef.
+
+(** * Correctness of sitpn_falling_edge function. *)
+
+Lemma sitpn_falling_edge_correct :
+  forall (sitpn : Sitpn)
+         (s s' : SitpnState)
+         (time_value : nat)
+         (env : Condition -> nat -> bool),
+    IsWellDefinedSitpn sitpn ->
+    IsWellDefinedSitpnState sitpn s ->
+    sitpn_falling_edge sitpn s time_value env = Some s' ->
+    SitpnSemantics sitpn s s' time_value env falling_edge.
+Proof.
+  intros sitpn s s' time_value env Hwell_def_sitpn Hwell_def_s Hfun.
+  apply SitpnSemantics_falling_edge.
+
+  (* CASE IsWellDefinedSitpn. *)
+  - assumption.
+
+  (* CASE IsWellDefinedSitpnState sitpn s. *)
+  - assumption.
+
+  (* CASE IsWellDefinedSitpnState sitpn s'. *)
+  - apply (sitpn_falling_edge_well_def_state
+             sitpn s s' time_value env Hwell_def_sitpn Hwell_def_s Hfun).
+
+  (* CASE marking s = marking s' *)
+  - admit.
+
+  (* CASE ∀ c ∈ C, cond'(c) = env(c) *)
+  - admit.
+
+  (* CASE ∀a ∈ A, ∃p ∈ P, ... ⇒ ex'(a) = 1. *)
+  - admit.
+
+  (* CASE ∀a ∈ A, ∀p ∈ P, ... ⇒ ex'(a) = 0. *)
+  - admit.
+
+  (* CASE reset(t) = 1 ∨ t ∈ Fired ⇒ I'(t) = Is(t) - 1 *)
+  - admit.
+
+  (* CASE reset(t) = 0 ∧ t ∉ Fired ∧ I(t) ≠ ψ ⇒ I'(t) = I(t) - 1 *)
+  - admit.
+
+  (* CASE reset(t) = 0 ∧ t ∉ Fired ∧ I(t) = ψ ⇒ I'(t) = I(t) *)
+  - admit.
+
+  (* CASE t ∉ sens(M) ⇒ I'(t) = Is(t) - 1 *)
+  - admit.
+
+  (* CASE reset s = reset s' *)
+  - admit.
+
+  (* CASE t ∉ firable(s') ⇒ t ∉ Fired' *)
+  - admit.
+
+  (* CASE t ∈ firable(s') ∧ t ∈ sens(M -∑pre) ⇒ t ∈ Fired' *)
+  - admit.
+
+  (* CASE t ∈ firable(s') ∧ t ∉ sens(M -∑pre) ⇒ t ∉ Fired' *)
+  - admit.
+    
+Admitted.
+
