Sitpn/SitpnFallingEdgeWellDef.v
@@ -1,0 +1,111 @@
+(* Import Sitpn material. *)
+
+Require Import Hilecop.Sitpn.Sitpn.
+Require Import Hilecop.Sitpn.SitpnTokenPlayer.
+Require Import Hilecop.Sitpn.SitpnSemantics.
+
+(* Import lemmas on synchronous execution rules. *)
+
+Require Import Hilecop.Sitpn.SitpnFallingEdgeFired.
+
+(* Import Sitpn tactics. *)
+
+Require Import Hilecop.Sitpn.SitpnTactics.
+
+(* Import lemmas on time rules. *)
+
+Require Import Hilecop.Sitpn.SitpnFallingEdgeTime.
+
+(** * sitpn_falling_edge and well-definedness of states. *)
+
+(** [sitpn_falling_edge] returns a SitpnState with the same marking 
+    as the starting state. *)
+
+Lemma sitpn_falling_edge_same_marking :
+  forall (sitpn : Sitpn)
+         (s s' : SitpnState)
+         (time_value : nat)
+         (env : Condition -> nat -> bool),
+    sitpn_falling_edge sitpn s time_value env = Some s' ->
+    (marking s) = (marking s').
+Proof.
+  intros sitpn s s' time_value env Hfun.
+  functional induction (sitpn_falling_edge sitpn s time_value env)
+             using sitpn_falling_edge_ind.
+
+  (* GENERAL CASE, all went well. *)
+  - simpl in Hfun; injection Hfun as Heq_s'; rewrite <- Heq_s'.
+    simpl; reflexivity.
+
+  (* ERROR CASE *)
+  - inversion Hfun.
+
+  (* ERROR CASE *)
+  - inversion Hfun.
+Qed.
+  
+(** [sitpn_falling_edge] returns a SitpnState that is well-defined. *)
+
+Lemma sitpn_falling_edge_well_def_state :
+  forall (sitpn : Sitpn)
+         (s s' : SitpnState)
+         (time_value : nat)
+         (env : Condition -> nat -> bool),
+    IsWellDefinedSitpn sitpn ->
+    IsWellDefinedSitpnState sitpn s ->
+    sitpn_falling_edge sitpn s time_value env = Some s' ->
+    IsWellDefinedSitpnState sitpn s'.
+Proof.
+  intros sitpn s s' time_value env Hwell_def_sitpn Hwell_def_s Hfun.
+  unfold IsWellDefinedSitpnState.
+  
+  (* CASE incl (fired s') (transs sitpn) *)
+  split.
+  apply (sitpn_falling_edge_incl_fired
+           sitpn s s' time_value env Hwell_def_sitpn Hfun).
+
+  (* CASE NoDup (fired s') *)
+  split.
+  apply (sitpn_falling_edge_nodup_fired
+           sitpn s s' time_value env Hwell_def_sitpn Hfun).           
+
+  (* CASE places = fst (split (marking s')) *)
+  split.
+  explode_well_defined_sitpn_state Hwell_def_s.
+  specialize (sitpn_falling_edge_same_marking sitpn s s' time_value env Hfun) as Heq_m.
+  rewrite <- Heq_m; assumption.
+
+  (* CASE t ∈ (d_intervals s') ⇔ t ∈ Ti *)
+  split.
+  explode_well_defined_sitpn_state Hwell_def_s.
+  revert t.
+  specialize (sitpn_falling_edge_same_struct_ditvals sitpn s s' time_value env Hfun)
+    as Heq_fs_ditvals.
+  rewrite <- Heq_fs_ditvals; assumption.
+
+  (* CASE NoDup (fst (split (d_intervals s'))) *)
+  split.
+  explode_well_defined_sitpn_state Hwell_def_s.
+  specialize (sitpn_falling_edge_same_struct_ditvals sitpn s s' time_value env Hfun)
+    as Heq_fs_ditvals.
+  rewrite <- Heq_fs_ditvals; assumption.
+
+  (* CASE t ∈ (reset s') ⇔ t ∈ Ti *)
+  split.
+  admit.
+
+  (* CASE NoDup (fst (split (reset s'))) *)
+  split.
+  admit.
+
+  (* CASE C = fst (split (cond_values s')) *)
+  split.
+  admit.
+
+  (* CASE A = fst (split (exec_a s')) *)
+  split.
+  admit.
+
+  (* CASE F = fst (split (exec_f s')) *)
+  admit.
+Admitted.
