Sitpn/SitpnRisingEdgeCorrect.v
@@ -1,0 +1,20 @@
+(* Import Sitpn material. *)
+
+Require Import Hilecop.Sitpn.Sitpn.
+Require Import Hilecop.Sitpn.SitpnTokenPlayer.
+Require Import Hilecop.Sitpn.SitpnSemantics.
+
+
+(** * Correctness of sitpn_rising_edge function. *)
+
+Lemma sitpn_rising_edge_correct :
+  forall (sitpn : Sitpn)
+         (s s' : SitpnState)
+         (time_value : nat)
+         (env : Condition -> nat -> bool),
+    IsWellDefinedSitpn sitpn ->
+    IsWellDefinedSitpnState sitpn s ->
+    sitpn_rising_edge sitpn s = Some s' ->
+    SitpnSemantics sitpn s s' time_value env rising_edge.
+Proof.
+Admitted.
