Sitpn/SitpnTactics.v
@@ -1,0 +1,152 @@
+Require Import Hilecop.Sitpn.Sitpn.
+
+(** Renames all hypotheses resulting of the decomposition 
+    of the IsWelldefinedSitpn predicate. *)
+
+Ltac rename_well_defined_sitpn :=
+  match goal with
+  | [ H: NoDupPlaces ?sitpn |- _ ] =>
+    rename H into Hnodup_places
+  end;
+  match goal with
+  | [ H: NoDupTranss ?sitpn |- _ ] =>
+    rename H into Hnodup_transs
+  end;
+  match goal with
+  | [ H: NoUnknownInPriorityGroups ?sitpn |- _ ] =>
+    rename H into Hno_unk_pgroups
+  end;
+  match goal with
+  | [ H: NoIntersectInPriorityGroups ?sitpn |- _ ] =>
+    rename H into Hno_inter
+  end;
+  match goal with
+  | [ H: AreWellFormedTimeIntervals ?sitpn |- _ ] =>
+    rename H into Hwell_formed_itvals
+  end;
+  match goal with
+  | [ H: NoDupConditions ?sitpn |- _ ] =>
+    rename H into Hnodup_cond
+  end;
+  match goal with
+  | [ H: NoDupActions ?sitpn |- _ ] =>
+    rename H into Hnodup_ac
+  end;
+  match goal with
+  | [ H: NoDupFunctions ?sitpn |- _ ] =>
+    rename H into Hnodup_fun
+  end;
+  match goal with
+  | [ H: NoDupInNeighbours ?sitpn |- _ ] =>
+    rename H into Hnodup_neigh
+  end;
+  match goal with
+  | [ H: NoIsolatedPlace ?sitpn |- _ ] =>
+    rename H into Hiso_place
+  end;
+  match goal with
+  | [ H: NoUnknownPlaceInNeighbours ?sitpn |- _ ] =>
+    rename H into Hunk_pl_neigh
+  end;
+  match goal with
+  | [ H: NoIsolatedTrans ?sitpn |- _ ] =>
+    rename H into Hiso_trans
+  end;
+  match goal with
+  | [ H: AreWellDefinedPreEdges ?sitpn |- _ ] =>
+    rename H into Hwell_def_pre
+  end;
+  match goal with
+  | [ H: AreWellDefinedTestEdges ?sitpn |- _ ] =>
+    rename H into Hwell_def_test
+  end;
+  match goal with
+  | [ H: AreWellDefinedInhibEdges ?sitpn |- _ ] =>
+    rename H into Hwell_def_inhib
+  end;
+  match goal with
+  | [ H: AreWellDefinedPostEdges ?sitpn |- _ ] =>
+    rename H into Hwell_def_post
+  end.
+
+Ltac explode_well_defined_sitpn :=
+  match goal with
+  | [ H: IsWellDefinedSitpn _ |- _ ] =>
+    assert (H' := H); 
+    unfold IsWellDefinedSitpn in H;
+    decompose [and] H;
+    intros;
+    rename_well_defined_sitpn;
+    clear H;
+    rename H' into Hwell_def_sitpn
+  end.
+
+(** Renames all hypotheses resulting of the decomposition
+    of IsWellDefinedSitpnState. *)
+
+Ltac rename_well_defined_sitpn_state :=
+  match goal with
+  | [ H: incl ?s.(Sitpn.fired) (transs ?sitpn) |- _ ] =>
+    rename H into Hincl_state_fired_transs
+  end;
+  match goal with
+  | [ H: NoDup ?s.(Sitpn.fired) |- _ ] =>
+    rename H into Hnodup_state_fired
+  end;
+  match goal with
+  | [ H: ?sitpn.(Sitpn.places) = fst (split (Sitpn.marking ?s))
+      |- _ ] =>
+    rename H into Hwf_state_marking
+  end;
+  match goal with
+  | [ H: (forall (t : Trans),
+             In t ?sitpn.(Sitpn.transs) /\
+             (Sitpn.s_intervals ?sitpn t) <> None <->
+             In t (fst (split ?s.(Sitpn.d_intervals))))
+      |- _ ] =>
+    rename H into Hwf_state_ditvals
+  end;
+  match goal with
+  | [ H: NoDup (fst (split (Sitpn.d_intervals ?s))) |- _ ] =>
+    rename H into Hnodup_state_ditvals
+  end;
+  match goal with
+  | [ H: (forall (t : Trans),
+             In t ?sitpn.(Sitpn.transs) /\
+             (Sitpn.s_intervals ?sitpn t) <> None <->
+             In t (fst (split ?s.(Sitpn.reset))))
+      |- _ ] =>
+    rename H into Hwf_state_reset
+  end;
+  match goal with
+  | [ H: NoDup (fst (split (Sitpn.reset ?s))) |- _ ] =>
+    rename H into Hnodup_state_reset
+  end;
+  match goal with
+  | [ H: (Sitpn.conditions ?sitpn) = fst (split (Sitpn.cond_values ?s))
+      |- _ ] =>
+    rename H into Hwf_state_condv
+  end;
+  match goal with
+  | [ H: (Sitpn.actions ?sitpn) = fst (split (Sitpn.exec_a ?s))
+      |- _ ] =>
+    rename H into Hwf_state_execa
+  end;
+  match goal with
+  | [ H: (Sitpn.functions ?sitpn) = fst (split (Sitpn.exec_f ?s))
+      |- _ ] =>
+    rename H into Hwf_state_execf
+  end.
+
+Ltac explode_well_defined_sitpn_state H :=
+  match H with
+  | H : IsWellDefinedSitpnState _ _  =>
+    assert (H' := H); 
+    unfold IsWellDefinedSitpnState in H;
+    decompose [and] H;
+    intros;
+    rename_well_defined_sitpn_state;
+    clear H;
+    rename H' into Hwell_def_state
+  | _ => fail "No predicate IsWellDefinedSitpnState found"
+  end.
